More abstract map types

src/CDCL/Impl.v
@@ -5,6 +5,8 @@ Import ListNotations.
 Require Import Stdlib.Arith.PeanoNat.
 Require Import Stdlib.Arith.Arith.
 Require Import Stdlib.micromega.Lia.
+Require Import FMV.FiniteMap.
+Require Import FMV.ListMap.
 
 Definition Var := nat.
 Variant Literal :=
@@ -28,425 +30,39 @@ Defined.
 Definition clause_eq_dec : forall l r : Clause, {l = r} + {l <> r} :=
   list_eq_dec literal_eq_dec.
 
-Module Type ClauseMapSig.
-  Parameter t : Type.
+Module VarKey.
+  Definition t := Var.
+  Definition eq_dec := Nat.eq_dec.
+End VarKey.
 
-  Parameter empty : t.
-  Parameter find : Var -> t -> list Clause.
-  Parameter keys : t -> list Var.
-  Parameter add : Var -> Clause -> t -> t.
-  Parameter remove : Var -> t -> t.
-  Parameter remove_clause : Clause -> t -> t.
-  Parameter card_of : Clause -> t -> nat.
-  Parameter elements : t -> list Clause.
+Module ClauseElement.
+  Definition t := Clause.
+  Definition eq_dec := clause_eq_dec.
+End ClauseElement.
 
-  Axiom find_empty : forall v, find v empty = [].
-  Axiom card_of_empty : forall c, card_of c empty = 0.
-  Axiom keys_complete : forall m v, find v m <> [] <-> In v (keys m).
-  Axiom find_add : forall m c d v x,
-    In d (find x (add v c m)) <->
-    (x = v /\ d = c) \/ In d (find x m).
-  Axiom find_add_eq : forall m c v x,
-    find x (add v c m) =
-      if Nat.eq_dec v x then c :: find x m else find x m.
-  Axiom card_of_add : forall m c v,
-    card_of c (add v c m) = S (card_of c m).
-  Axiom card_of_add_neq : forall m c d v,
-    c <> d -> card_of d (add v c m) = card_of d m.
-  Axiom card_of_remove : forall m c v,
-    card_of c (remove v m) + count_occ clause_eq_dec (find v m) c =
-      card_of c m.
-  Axiom card_of_remove_clause_eq : forall m c,
-    card_of c (remove_clause c m) = 0.
-  Axiom card_of_remove_clause_neq : forall m c d,
-    c <> d -> card_of d (remove_clause c m) = card_of d m.
-  Axiom card_of_unique : forall m c v v',
-    card_of c m = 1 -> In c (find v m) -> In c (find v' m) -> v = v'.
-  Axiom card_of_in : forall m c v, In c (find v m) -> card_of c m > 0.
-  Axiom find_remove : forall m v d v',
-    In d (find v (remove v' m)) <-> In d (find v m) /\ v <> v'.
-  Axiom find_remove_eq : forall m v v',
-    find v (remove v' m) =
-      if Nat.eq_dec v' v then [] else find v m.
-  Axiom find_remove_clause : forall m c d v,
-    In d (find v (remove_clause c m)) <-> In d (find v m) /\ d <> c.
-  Axiom find_remove_clause_eq : forall m c v,
-    find v (remove_clause c m) =
-      filter (fun c' => if clause_eq_dec c c' then false else true) (find v m).
-  Axiom elements_spec : forall m c,
-    In c (elements m) <-> exists v, In v (keys m) /\ In c (find v m).
-End ClauseMapSig.
+Module ClauseMapBase := ListMap.Make VarKey ClauseElement.
 
-(* Clauses indexed by variable. An empty list represents an absent entry. An
-   explicit support makes it possible to enumerate the finite map. *)
-Module ClauseMap : ClauseMapSig.
-  Record representation := make {
-      lookup : Var -> list Clause;
-      support : list Var;
-      support_spec : NoDup support /\
-        forall v, lookup v <> [] <-> In v support
-    }.
-  Definition t := representation.
+Module ClauseMap.
+  Include ClauseMapBase.
 
-  Definition find (v : Var) (m : t) : list Clause := m.(lookup) v.
-  Definition keys (m : t) : list Var := m.(support).
-
-  Definition empty : t.
-  Proof.
-    refine {| lookup := fun _ => []; support := [] |}.
-    split; [constructor|]. intros v. split; intros H; contradiction.
-  Defined.
-
-  Definition add (v : Var) (c : Clause) (m : t) : t.
-  Proof.
-    refine
-      {| lookup := fun v' =>
-           if Nat.eq_dec v v' then c :: m.(lookup) v' else m.(lookup) v';
-         support := if in_dec Nat.eq_dec v m.(support)
-           then m.(support) else v :: m.(support) |}.
-    split.
-    - destruct (in_dec Nat.eq_dec v m.(support)).
-      + exact (proj1 m.(support_spec)).
-      + constructor; [assumption|exact (proj1 m.(support_spec))].
-    - intros v'.
-    destruct (Nat.eq_dec v v') as [-> | Hneq].
-      + simpl. split; [|intros _; discriminate].
-        intros _. destruct (in_dec Nat.eq_dec v' m.(support)); [assumption|now left].
-      + simpl. destruct (Nat.eq_dec v v') as [Heq | _]; [contradiction|].
-        rewrite (proj2 m.(support_spec) v').
-        destruct (in_dec Nat.eq_dec v m.(support)); simpl; intuition congruence.
-  Defined.
-
-  Definition remove_from (c : Clause) (cs : list Clause) : list Clause :=
-    filter (fun c' => if clause_eq_dec c c' then false else true) cs.
-
-  Definition nonempty (cs : list Clause) : bool :=
-    match cs with
-    | [] => false
-    | _ :: _ => true
-    end.
-
-  Definition remove (v : Var) (m : t) : t.
-  Proof.
-    refine
-      {| lookup := fun v' => if Nat.eq_dec v v' then [] else m.(lookup) v';
-         support := filter (fun v' => negb (Nat.eqb v v')) m.(support) |}.
-    split; [apply NoDup_filter; exact (proj1 m.(support_spec))|].
-    intros v'.
-    destruct (Nat.eq_dec v v') as [->|Hneq].
-    - simpl. split.
-      + intros H. contradiction.
-      + intros H. apply filter_In in H as [_ Hneqb].
-        rewrite Nat.eqb_refl in Hneqb. discriminate.
-    - assert (Nat.eqb v v' = false) as Heqb by now apply Nat.eqb_neq.
-      simpl. destruct (Nat.eq_dec v v') as [Heq|_]; [contradiction|].
-      rewrite filter_In, Heqb. simpl.
-      rewrite (proj2 m.(support_spec) v'). tauto.
-  Defined.
-
-  Definition remove_clause (c : Clause) (m : t) : t.
-  Proof.
-    refine
-      {| lookup := fun v =>
-           remove_from c (m.(lookup) v);
-         support := filter
-           (fun v => nonempty (remove_from c (m.(lookup) v)))
-           m.(support) |}.
-    split; [apply NoDup_filter; exact (proj1 m.(support_spec))|].
-    intros v. split.
-    - intros H.
-      apply filter_In. split.
-      + apply (proj2 m.(support_spec)). intro Heq.
-        rewrite Heq in H. exact (H eq_refl).
-      + destruct (remove_from c (m.(lookup) v)); [contradiction|reflexivity].
-    - intros H.
-      apply filter_In in H as [_ Hnonempty].
-      destruct (remove_from c (m.(lookup) v)); discriminate.
-  Defined.
-
-  Definition elements (m : t) : list Clause :=
-    flat_map m.(lookup) m.(support).
-
-  Definition card_of (c : Clause) (m : t) : nat :=
-    count_occ clause_eq_dec (elements m) c.
-
-  Lemma find_empty : forall v, find v empty = [].
-  Proof. reflexivity. Qed.
-
-  Lemma card_of_empty : forall c, card_of c empty = 0.
-  Proof. reflexivity. Qed.
-
-  Lemma keys_complete : forall m v, find v m <> [] <-> In v (keys m).
-  Proof. intros m v. exact (proj2 m.(support_spec) v). Qed.
-
-  Lemma lookup_notin_support : forall m v,
-    ~ In v m.(support) -> m.(lookup) v = [].
-  Proof.
-    intros m v Hnotin. destruct (m.(lookup) v) as [|c cs] eqn:Hlookup;
-      [reflexivity|].
-    exfalso. apply Hnotin. apply (proj2 m.(support_spec) v).
-    rewrite Hlookup. discriminate.
-  Qed.
-
-  Lemma find_add : forall m c d v x,
-    In d (find x (add v c m)) <->
-    (x = v /\ d = c) \/ In d (find x m).
-  Proof.
-    intros m c d v x. unfold find, add. simpl.
-    destruct (Nat.eq_dec v x) as [->|Hneq]; simpl.
-    - firstorder.
-    - split; [now right|]. intros [[Heq _]|H]; [congruence|exact H].
-  Qed.
-
-  Lemma find_add_eq : forall m c v x,
-    find x (add v c m) =
-      if Nat.eq_dec v x then c :: find x m else find x m.
-  Proof. reflexivity. Qed.
-
-  Lemma count_occ_flat_map_add_absent : forall vs f v c d,
-    ~ In v vs ->
-    count_occ clause_eq_dec
-      (flat_map (fun x => if Nat.eq_dec v x then c :: f x else f x) vs) d =
-    count_occ clause_eq_dec (flat_map f vs) d.
-  Proof.
-    intros vs. induction vs as [|x xs IH]; intros f v c d Hnotin; simpl.
-    - reflexivity.
-    - destruct (Nat.eq_dec v x) as [->|Hneq].
-      + exfalso. apply Hnotin. now left.
-      +
-      rewrite !count_occ_app. rewrite IH; [reflexivity|].
-      now intros Hin; apply Hnotin; right.
-  Qed.
-
-  Lemma count_occ_flat_map_add_present : forall vs f v c d,
-    NoDup vs -> In v vs ->
-    count_occ clause_eq_dec
-      (flat_map (fun x => if Nat.eq_dec v x then c :: f x else f x) vs) d =
-    count_occ clause_eq_dec [c] d +
-      count_occ clause_eq_dec (flat_map f vs) d.
-  Proof.
-    intros vs. induction vs as [|x xs IH]; intros f v c d Hnodup Hin;
-      [contradiction|].
-    inversion Hnodup as [|? ? Hnotin Hnodup']; subst.
-    simpl in Hin. cbn [flat_map].
-    destruct (Nat.eq_dec v x) as [->|Hneq].
-    - destruct (Nat.eq_dec x x) as [_|Habs]; [|contradiction].
-      rewrite !count_occ_app.
-      rewrite (count_occ_flat_map_add_absent xs f x c d Hnotin).
-      destruct (clause_eq_dec c d) eqn:Hcd; simpl; rewrite Hcd; simpl; lia.
-    - destruct (Nat.eq_dec v x) as [Habs|_]; [contradiction|].
-      rewrite !count_occ_app, IH; [lia|exact Hnodup'|].
-      destruct Hin as [Heq|Hin]; [congruence|exact Hin].
-  Qed.
-
-  Lemma card_of_add : forall m c v,
-    card_of c (add v c m) = S (card_of c m).
-  Proof.
-    intros m c v. unfold card_of, elements, add. simpl.
-    destruct (in_dec Nat.eq_dec v m.(support)) as [Hin|Hnotin].
-    - rewrite count_occ_flat_map_add_present;
-        [|exact (proj1 m.(support_spec))|exact Hin].
-      simpl. destruct (clause_eq_dec c c) eqn:Hcc;
-        [simpl; reflexivity|contradiction].
-    - simpl. destruct (Nat.eq_dec v v) as [_|Habs]; [|contradiction].
-      rewrite (lookup_notin_support m v Hnotin).
-      rewrite !count_occ_app, count_occ_flat_map_add_absent by exact Hnotin.
-      simpl. destruct (clause_eq_dec c c) eqn:Hcc;
-        [simpl; reflexivity|contradiction].
-  Qed.
-
-  Lemma card_of_add_neq : forall m c d v,
-    c <> d -> card_of d (add v c m) = card_of d m.
-  Proof.
-    intros m c d v Hneq. unfold card_of, elements, add. simpl.
-    destruct (in_dec Nat.eq_dec v m.(support)) as [Hin|Hnotin].
-    - rewrite count_occ_flat_map_add_present;
-        [|exact (proj1 m.(support_spec))|exact Hin].
-      simpl. destruct (clause_eq_dec c d) eqn:Hcd;
-        [contradiction|simpl; reflexivity].
-    - simpl. destruct (Nat.eq_dec v v) as [_|Habs]; [|contradiction].
-      rewrite (lookup_notin_support m v Hnotin).
-      rewrite !count_occ_app, count_occ_flat_map_add_absent by exact Hnotin.
-      simpl. destruct (clause_eq_dec c d) eqn:Hcd;
-        [contradiction|simpl; reflexivity].
-  Qed.
-
-  Lemma filter_remove_absent : forall vs v,
-    ~ In v vs -> filter (fun v' => negb (Nat.eqb v v')) vs = vs.
-  Proof.
-    intros vs. induction vs as [|x xs IH]; intros v Hnotin; simpl.
-    - reflexivity.
-    - destruct (v =? x) eqn:Heq.
-      + apply Nat.eqb_eq in Heq. subst. exfalso. apply Hnotin. now left.
-      + simpl. f_equal. apply IH. intros Hin. apply Hnotin. now right.
-  Qed.
-
-  Lemma flat_map_remove_absent : forall (vs : list Var)
-      (f : Var -> list Clause) v,
-    ~ In v vs ->
-    flat_map (fun x => if Nat.eq_dec v x then [] else f x) vs = flat_map f vs.
-  Proof.
-    intros vs. induction vs as [|x xs IH]; intros f v Hnotin; simpl.
-    - reflexivity.
-    - destruct (Nat.eq_dec v x) as [->|Hneq].
-      + exfalso. apply Hnotin. now left.
-      + f_equal. apply IH. intros Hin. apply Hnotin. now right.
-  Qed.
-
-  Lemma card_of_remove : forall m c v,
-    card_of c (remove v m) + count_occ clause_eq_dec (find v m) c =
-      card_of c m.
-  Proof.
-    intros m c v. unfold card_of, elements, find, remove. simpl.
-    destruct (in_dec Nat.eq_dec v m.(support)) as [Hin|Hnotin].
-    - apply in_split in Hin as [before [after Hsupport]].
-      pose proof (proj1 m.(support_spec)) as Hnodup.
-      rewrite Hsupport in Hnodup |- *.
-      rewrite filter_app. simpl. rewrite Nat.eqb_refl. simpl.
-      pose proof (NoDup_remove_2 _ _ _ Hnodup) as Hnotin_rest.
-      assert (~ In v before) as Hnotin_before.
-      { intros H. apply Hnotin_rest. apply in_or_app. now left. }
-      assert (~ In v after) as Hnotin_after.
-      { intros H. apply Hnotin_rest. apply in_or_app. now right. }
-      rewrite (filter_remove_absent before v Hnotin_before).
-      rewrite (filter_remove_absent after v Hnotin_after).
-      rewrite !flat_map_app.
-      erewrite flat_map_remove_absent by exact Hnotin_before.
-      erewrite flat_map_remove_absent by exact Hnotin_after.
-      cbn [flat_map]. rewrite !count_occ_app.
-      set (nb := count_occ clause_eq_dec (flat_map m.(lookup) before) c).
-      set (nv := count_occ clause_eq_dec (m.(lookup) v) c).
-      set (na := count_occ clause_eq_dec (flat_map m.(lookup) after) c).
-      change (nb + na + nv = nb + (nv + na)). lia.
-    - rewrite (filter_remove_absent m.(support) v Hnotin).
-      erewrite flat_map_remove_absent by exact Hnotin.
-      rewrite (lookup_notin_support m v Hnotin). simpl. lia.
-  Qed.
-
-  Lemma flat_map_filter_nonempty : forall (vs : list Var)
-      (f : Var -> list Clause),
-    flat_map f (filter (fun v => nonempty (f v)) vs) = flat_map f vs.
-  Proof.
-    intros vs. induction vs as [|v vs IH]; intros f; simpl.
-    - reflexivity.
-    - destruct (f v) as [|x xs] eqn:Hf; simpl.
-      + rewrite IH. reflexivity.
-      + rewrite Hf, IH. reflexivity.
-  Qed.
-
-  Lemma count_occ_remove_from_eq : forall cs c,
-    count_occ clause_eq_dec (remove_from c cs) c = 0.
-  Proof.
-    intros cs. induction cs as [|d cs IH]; intros c; simpl.
-    - reflexivity.
-    - destruct (clause_eq_dec c d) as [->|Hneq]; simpl.
-      + exact (IH d).
-      + destruct (clause_eq_dec d c) as [Heq|_]; [congruence|]. exact (IH c).
-  Qed.
-
-  Lemma count_occ_remove_from_neq : forall cs c d,
-    c <> d ->
-    count_occ clause_eq_dec (remove_from c cs) d = count_occ clause_eq_dec cs d.
-  Proof.
-    intros cs. induction cs as [|x xs IH]; intros c d Hneq; simpl.
-    - reflexivity.
-    - destruct (clause_eq_dec c x) as [->|Hcx]; simpl.
-      + destruct (clause_eq_dec x d) as [Heq|_]; [congruence|].
-        apply IH. exact Hneq.
-      + destruct (clause_eq_dec x d); simpl; rewrite IH by exact Hneq;
-          reflexivity.
-  Qed.
+  Definition remove_clause := remove_element.
 
   Lemma card_of_remove_clause_eq : forall m c,
     card_of c (remove_clause c m) = 0.
-  Proof.
-    intros m c. unfold card_of, elements, remove_clause. simpl.
-    rewrite flat_map_filter_nonempty.
-    induction m.(support) as [|v vs IH]; simpl; [reflexivity|].
-    rewrite count_occ_app, count_occ_remove_from_eq, IH. reflexivity.
-  Qed.
+  Proof. exact card_of_remove_element_eq. Qed.
 
   Lemma card_of_remove_clause_neq : forall m c d,
     c <> d -> card_of d (remove_clause c m) = card_of d m.
-  Proof.
-    intros m c d Hneq. unfold card_of, elements, remove_clause. simpl.
-    rewrite flat_map_filter_nonempty.
-    induction m.(support) as [|v vs IH]; simpl; [reflexivity|].
-    rewrite !count_occ_app, count_occ_remove_from_neq by exact Hneq.
-    now rewrite IH.
-  Qed.
-
-  Lemma card_of_unique : forall m c v v',
-    card_of c m = 1 -> In c (find v m) -> In c (find v' m) -> v = v'.
-  Proof.
-    intros m c v v' Hcard Hv Hv'. destruct (Nat.eq_dec v v') as [->|Hneq];
-      [reflexivity|exfalso].
-    assert (In v m.(support)) as Hvs.
-    { apply keys_complete. intro Hempty. rewrite Hempty in Hv. contradiction. }
-    assert (In v' m.(support)) as Hvs'.
-    { apply keys_complete. intro Hempty. rewrite Hempty in Hv'. contradiction. }
-    apply in_split in Hvs as [before [after Hsupport]].
-    assert (In v' (before ++ after)) as Hv'rest.
-    { rewrite Hsupport in Hvs'.
-      apply in_app_or in Hvs' as [Hin|Hin].
-      - now apply in_or_app; left.
-      - simpl in Hin. destruct Hin as [Heq|Hin]; [congruence|].
-        now apply in_or_app; right. }
-    assert (In c (flat_map m.(lookup) (before ++ after))) as Hcrest.
-    { apply in_flat_map. exists v'. split; [exact Hv'rest|exact Hv']. }
-    unfold find in Hv, Hv'.
-    apply (proj1 (count_occ_In clause_eq_dec _ _)) in Hv.
-    apply (proj1 (count_occ_In clause_eq_dec _ _)) in Hcrest.
-    unfold card_of, elements, find in Hcard, Hv'.
-    rewrite Hsupport, flat_map_app in Hcard. cbn [flat_map] in Hcard.
-    rewrite !count_occ_app in Hcard.
-    rewrite flat_map_app, count_occ_app in Hcrest. lia.
-  Qed.
-
-  Lemma card_of_in : forall m c v, In c (find v m) -> card_of c m > 0.
-  Proof.
-    intros m c v Hin. unfold card_of. apply count_occ_In.
-    unfold elements. apply in_flat_map. exists v. split; [|exact Hin].
-    apply keys_complete.
-    intros Hempty. rewrite Hempty in Hin. contradiction.
-  Qed.
-
-  Lemma find_remove : forall m v d v',
-    In d (find v (remove v' m)) <-> In d (find v m) /\ v <> v'.
-  Proof.
-    intros m v d v'. unfold find, remove. simpl.
-    destruct (Nat.eq_dec v' v) as [->|Hneq].
-    - simpl. firstorder.
-    - simpl. firstorder congruence.
-  Qed.
-
-  Lemma find_remove_eq : forall m v v',
-    find v (remove v' m) =
-      if Nat.eq_dec v' v then [] else find v m.
-  Proof. reflexivity. Qed.
+  Proof. exact card_of_remove_element_neq. Qed.
 
   Lemma find_remove_clause : forall m c d v,
     In d (find v (remove_clause c m)) <-> In d (find v m) /\ d <> c.
-  Proof.
-    intros m c d v. unfold find, remove_clause. simpl. unfold remove_from.
-    rewrite filter_In.
-    destruct (clause_eq_dec c d) as [->|Hneq].
-    - destruct (clause_eq_dec d d) as [_|Habs]; [|contradiction].
-      simpl. intuition congruence.
-    - destruct (clause_eq_dec c d) as [Habs|_]; [contradiction|].
-      simpl. intuition congruence.
-  Qed.
+  Proof. exact find_remove_element. Qed.
 
   Lemma find_remove_clause_eq : forall m c v,
     find v (remove_clause c m) =
       filter (fun c' => if clause_eq_dec c c' then false else true) (find v m).
-  Proof. reflexivity. Qed.
-
-  Lemma elements_spec : forall m c,
-    In c (elements m) <-> exists v, In v (keys m) /\ In c (find v m).
-  Proof.
-    intros m c. unfold elements, keys, find. apply in_flat_map.
-  Qed.
+  Proof. exact find_remove_element_eq. Qed.
 End ClauseMap.
 
 Record State := {
